deps/poulet4/lib/P4light/Semantics/Interpreter.v
@@ -562,6 +562,15 @@ Section Interpreter.
     Definition interp_call_copy_out (args : list (option Lval * direction)) (vals : list Sval) (s: state) : result Exn.t state :=
       interp_write_options s (filter_out args) vals.
 
+    Fixpoint expr_to_string {tags_t: Type} (e: @Expression tags_t) : string :=
+      match e with
+      | MkExpression _ (ExpName _ loc) _ _ =>
+          Exn.loc_to_string loc
+      | MkExpression _ (ExpExpressionMember expr name) _ _ =>
+          expr_to_string expr ++ "." ++ str name
+      | _ => "<expr>"
+      end.
+
     Fixpoint interp_stmt (this: path) (st: state) (fuel: Fuel) (stmt: @Statement tags_t) : result Exn.t (state * signal) :=
       match fuel with
       | NoFuel => error (Exn.Other "interp_func: no fuel")
@@ -706,7 +715,10 @@ Section Interpreter.
                    else let dirs := get_arg_directions func in
                         let* (argvals, sig) := interp_args this st args dirs in
                         let* (obj_path, fd) := from_opt (lookup_func ge this func)
-                                                        (Exn.Other "lookup_func") in
+                                                        (Exn.Other ("interp_stmt: lookup_func could not find "
+                                                                      ++ Exn.path_to_string this
+                                                                      ++ "."
+                                                                      ++ expr_to_string func)) in
                         let s2 := if is_some obj_path then set_memory PathMap.empty st else st in
                         let* (s3, outvals, sig') := interp_func (force this obj_path) s2 fuel fd targs (extract_invals argvals) in
                         let s4 := if is_some obj_path then set_memory (get_memory st) s3 else s3 in
@@ -767,6 +779,7 @@ Section Interpreter.
                    let args' := List.map eval_val_to_sval argvs' in
                    mret ((m, es'), args', sig)
                end
+
            end.
 
     (* Analogue of exec_module *)
